compiler/eval/compilerComputeLib.sml
@@ -381,6 +381,8 @@ val add_compiler_compset = computeLib.extend_compset
     ,data_to_wordTheory.RefArray_location_eq
     ,data_to_wordTheory.Replicate_location_eq
     ,data_to_wordTheory.AllocVar_def
+    ,data_to_wordTheory.MakeBytes_def
+    ,data_to_wordTheory.SmallLsr_def
     ,data_to_wordTheory.RefByte_code_def
     ,data_to_wordTheory.FromList_code_def
     ,data_to_wordTheory.FromList1_code_def
